src/Analysis/Domains/Sign_Side_Soundness.thy
@@ -34,7 +34,7 @@ text \<open>
 \<close>
 
 lemma sign_sound_etf:
-  "sound_effectful_transfer gamma_sign sign_etf"
+  "sound_effectful_transfer sign_etf"
   unfolding sign_etf_def
   by (rule sound_transfer_imp_sound_effectful[OF sign_sound_tf.sound_transfer_axioms])
 
@@ -62,7 +62,7 @@ theorem side_sign_analysis_sound:
   shows "t \<in> \<lbrakk>side_analyse_eff \<Pi> ps main sign_etf bot s0 ()
          (cfg_exit (compile_prog \<Pi> ps main))\<rbrakk>"
 proof -
-  interpret se: sound_effectful_transfer gamma_sign sign_etf
+  interpret se: sound_effectful_transfer sign_etf
     by (rule sign_sound_etf)
   have gs: "{s} \<le> \<lbrakk>s0\<rbrakk>"
     using s_sound by simp
