src/Analysis/Equations/Constraint_System_Sound.thy
@@ -33,7 +33,7 @@ proof -
   define edge_vals where
     "edge_vals = image (\<lambda>(u, a). apply_tf tf a (env u)) (predecessors g v)"
   define comb_vals where
-    "comb_vals = image (\<lambda>(c, e). combine_abs (env c) (env e)) (combine_predecessors g v)"
+    "comb_vals = image (\<lambda>(c, e). \<langle>env c|env e\<rangle>) (combine_predecessors g v)"
   define base where
     "base = (if v = cfg_entry g then insert s0 (edge_vals \<union> comb_vals)
             else edge_vals \<union> comb_vals)"
@@ -59,12 +59,12 @@ lemma combine_abs_le_rhs:
   assumes finE: "finite (edges g)"
   assumes finC: "finite (combines g)"
   assumes uce: "(c, e, v) \<in> combines g"
-  shows "combine_abs (env c) (env e) \<le> rhs g tf (\<squnion>) bot s0 env v"
+  shows "\<langle>env c|env e\<rangle> \<le> rhs g tf (\<squnion>) bot s0 env v"
 proof -
   define edge_vals where
     "edge_vals = image (\<lambda>(u, a). apply_tf tf a (env u)) (predecessors g v)"
   define comb_vals where
-    "comb_vals = image (\<lambda>(c, e). combine_abs (env c) (env e)) (combine_predecessors g v)"
+    "comb_vals = image (\<lambda>(c, e). \<langle>env c|env e\<rangle>) (combine_predecessors g v)"
   define base where
     "base = (if v = cfg_entry g then insert s0 (edge_vals \<union> comb_vals)
             else edge_vals \<union> comb_vals)"
@@ -74,9 +74,9 @@ proof -
     unfolding comb_vals_def using finC by (simp add: finite_combine_predecessors)
   have fin_base: "finite base"
     unfolding base_def using fin_edge fin_comb by simp
-  have mem_base: "combine_abs (env c) (env e) \<in> base"
+  have mem_base: "\<langle>env c|env e\<rangle> \<in> base"
     using uce unfolding base_def comb_vals_def combine_predecessors_def by auto
-  have "combine_abs (env c) (env e) \<le> abs_join_set (\<squnion>) bot base"
+  have "\<langle>env c|env e\<rangle> \<le> abs_join_set (\<squnion>) bot base"
     using sup_fold_ge_state[OF fin_base mem_base] unfolding abs_join_set_def by simp
   also have "\<dots> = rhs g tf (\<squnion>) bot s0 env v"
     unfolding rhs_def Let_def base_def edge_vals_def comb_vals_def
@@ -94,7 +94,7 @@ proof -
   define edge_vals where
     "edge_vals = image (\<lambda>(u, a). apply_tf tf a (env u)) (predecessors g (cfg_entry g))"
   define comb_vals where
-    "comb_vals = image (\<lambda>(c, e). combine_abs (env c) (env e)) (combine_predecessors g (cfg_entry g))"
+    "comb_vals = image (\<lambda>(c, e). \<langle>env c|env e\<rangle>) (combine_predecessors g (cfg_entry g))"
   define base where "base = insert s0 (edge_vals \<union> comb_vals)"
   have fin_edge: "finite edge_vals"
     unfolding edge_vals_def using finE by (simp add: finite_predecessors)
@@ -113,13 +113,15 @@ qed
 
 subsection \<open>Per-step soundness and the main theorem\<close>
 
+subsection \<open>Per-step soundness and the main theorem\<close>
+
 context sound_transfer
 begin
 
 (* Per-edge soundness: edge_collect on concretisation factors through
    apply_tf in the abstract domain. *)
 lemma edge_collect_apply_tf_sound:
-  shows "edge_collect a (gamma_state \<sigma>) \<subseteq> gamma_state (apply_tf tf a \<sigma>)"
+  shows "edge_collect a \<lbrakk>\<sigma>\<rbrakk> \<subseteq> \<lbrakk>apply_tf tf a \<sigma>\<rbrakk>"
 proof (cases a)
   case EA_Nop
   then show ?thesis by simp
@@ -149,20 +151,20 @@ lemma collect_pp_abstract_sound:
   assumes fin: "finite (edges g)"
   assumes finC: "finite (combines g)"
   assumes post_fp: "is_post_fixpoint g tf (\<squnion>) bot s0 env"
-  shows "collect_pp g (\<lambda>v. gamma_state (env v)) v \<subseteq> gamma_state (env v)"
+  shows "collect_pp g (\<lambda>v. \<lbrakk>env v\<rbrakk>) v \<subseteq> \<lbrakk>env v\<rbrakk>"
 proof
   fix x
-  assume xin: "x \<in> collect_pp g (\<lambda>v. gamma_state (env v)) v"
+  assume xin: "x \<in> collect_pp g (\<lambda>v. \<lbrakk>env v\<rbrakk>) v"
   then obtain u a where uav: "(u, a, v) \<in> edges g"
-    and xin': "x \<in> edge_collect a (gamma_state (env u))"
+    and xin': "x \<in> edge_collect a \<lbrakk>env u\<rbrakk>"
     unfolding collect_pp_def by blast
-  have step1: "x \<in> gamma_state (apply_tf tf a (env u))"
+  have step1: "x \<in> \<lbrakk>apply_tf tf a (env u)\<rbrakk>"
     using edge_collect_apply_tf_sound xin' by blast
   have le_rhs: "apply_tf tf a (env u) \<le> rhs g tf (\<squnion>) bot s0 env v"
     by (rule apply_tf_le_rhs[OF fin finC uav])
   have le_env: "rhs g tf (\<squnion>) bot s0 env v \<le> env v"
     using post_fp unfolding is_post_fixpoint_def by simp
-  show "x \<in> gamma_state (env v)"
+  show "x \<in> \<lbrakk>env v\<rbrakk>"
     using gamma_state_mono[OF order_trans[OF le_rhs le_env]] step1 by blast
 qed
 
@@ -170,25 +172,25 @@ lemma collect_combine_pp_abstract_sound:
   assumes fin: "finite (edges g)"
   assumes finC: "finite (combines g)"
   assumes post_fp: "is_post_fixpoint g tf (\<squnion>) bot s0 env"
-  shows "collect_combine_pp g (\<lambda>v. gamma_state (env v)) v
-         \<subseteq> gamma_state (env v)"
+  shows "collect_combine_pp g (\<lambda>v. \<lbrakk>env v\<rbrakk>) v
+         \<subseteq> \<lbrakk>env v\<rbrakk>"
 proof
   fix x
-  assume xin: "x \<in> collect_combine_pp g (\<lambda>v. gamma_state (env v)) v"
+  assume xin: "x \<in> collect_combine_pp g (\<lambda>v. \<lbrakk>env v\<rbrakk>) v"
   from xin obtain c ex ret s t where
         h: "(c, ex, ret) \<in> combines g" "ret = v"
-    and st: "s \<in> gamma_state (env c)" "t \<in> gamma_state (env ex)"
-    and x: "x = combine_states s t"
+    and st: "s \<in> \<lbrakk>env c\<rbrakk>" "t \<in> \<lbrakk>env ex\<rbrakk>"
+    and x: "x = <s|t>"
     unfolding collect_combine_pp_def by blast
-  have step: "x \<in> gamma_state (combine_abs (env c) (env ex))"
+  have step: "x \<in> \<lbrakk>\<langle>env c|env ex\<rangle>\<rbrakk>"
     using combine_states_sound[OF st] x by simp
   have uce: "(c, ex, v) \<in> combines g"
     using h(1,2) by force
-  have le_rhs: "combine_abs (env c) (env ex) \<le> rhs g tf (\<squnion>) bot s0 env v"
+  have le_rhs: "\<langle>env c|env ex\<rangle> \<le> rhs g tf (\<squnion>) bot s0 env v"
     by (rule combine_abs_le_rhs[OF fin finC uce])
   have le_env: "rhs g tf (\<squnion>) bot s0 env v \<le> env v"
     using post_fp unfolding is_post_fixpoint_def by simp
-  show "x \<in> gamma_state (env v)"
+  show "x \<in> \<lbrakk>env v\<rbrakk>"
     using gamma_state_mono[OF order_trans[OF le_rhs le_env]] step by blast
 qed
 
@@ -200,37 +202,37 @@ lemma cfg_witness_gamma:
     "\<And>u a w. (u, a, w) \<in> edges g \<Longrightarrow> apply_tf tf a (env u) \<le> env w"
   assumes combine_le:
     "\<And>c ex ret. (c, ex, ret) \<in> combines g \<Longrightarrow>
-       combine_abs (env c) (env ex) \<le> env ret"
+       \<langle>env c|env ex\<rangle> \<le> env ret"
   assumes entry_le: "s0 \<le> env (cfg_entry g)"
-  assumes S_le: "S \<le> gamma_state s0"
+  assumes S_le: "S \<le> \<lbrakk>s0\<rbrakk>"
   assumes wit: "cfg_witness g S v st"
-  shows "st \<in> gamma_state (env v)"
+  shows "st \<in> \<lbrakk>env v\<rbrakk>"
 proof -
-  from wit S_le show "st \<in> gamma_state (env v)"
+  from wit S_le show "st \<in> \<lbrakk>env v\<rbrakk>"
   proof (induction rule: cfg_witness.induct)
     case (entry v s Sa)
     show ?case using S_le entry_le gamma_state_mono entry by blast
   next
     case (edge u a v S s t)
-    have s_g: "s \<in> gamma_state (env u)" using edge by simp
+    have s_g: "s \<in> \<lbrakk>env u\<rbrakk>" using edge by simp
     have t_ec: "t \<in> edge_collect a {s}" using edge by simp
-    have step1: "t \<in> gamma_state (apply_tf tf a (env u))"
+    have step1: "t \<in> \<lbrakk>apply_tf tf a (env u)\<rbrakk>"
     proof -
-      have sub: "{s} \<subseteq> gamma_state (env u)" using s_g by simp
-      have ec: "edge_collect a (gamma_state (env u))
-        \<subseteq> gamma_state (apply_tf tf a (env u))"
+      have sub: "{s} \<subseteq> \<lbrakk>env u\<rbrakk>" using s_g by simp
+      have ec: "edge_collect a \<lbrakk>env u\<rbrakk>
+        \<subseteq> \<lbrakk>apply_tf tf a (env u)\<rbrakk>"
         using edge_collect_apply_tf_sound by blast
-      have "edge_collect a {s} \<subseteq> edge_collect a (gamma_state (env u))"
+      have "edge_collect a {s} \<subseteq> edge_collect a \<lbrakk>env u\<rbrakk>"
         using edge_collect_mono[OF sub] by blast
       thus ?thesis using t_ec ec by blast
     qed
     show ?case using gamma_state_mono[OF step_le[OF edge(1)]] step1 by blast
   next
     case (combine c ex v S s t)
-    have sc: "s \<in> gamma_state (env c)" and tc: "t \<in> gamma_state (env ex)"
+    have sc: "s \<in> \<lbrakk>env c\<rbrakk>" and tc: "t \<in> \<lbrakk>env ex\<rbrakk>"
       apply (auto simp add: combine.IH(1) combine.prems)
       by (simp add: combine.IH(2) combine.prems)
-    have step: "combine_states s t \<in> gamma_state (combine_abs (env c) (env ex))"
+    have step: "<s|t> \<in> \<lbrakk>\<langle>env c|env ex\<rangle>\<rbrakk>"
       using combine_states_sound[OF sc tc] by simp
     show ?case using gamma_state_mono[OF combine_le[OF combine(1)]] step by blast
   qed
@@ -241,14 +243,14 @@ lemma post_fixpoint_sound_at:
     and S :: "store set" and v0 :: pp
   assumes fin: "finite (edges g)"
   assumes finC: "finite (combines g)"
-  assumes S_sound: "S \<le> gamma_state s0"
+  assumes S_sound: "S \<le> \<lbrakk>s0\<rbrakk>"
   assumes step_le:
     "\<And>u a w. (u, a, w) \<in> edges g \<Longrightarrow> apply_tf tf a (env u) \<le> env w"
   assumes combine_le:
     "\<And>c ex ret. (c, ex, ret) \<in> combines g \<Longrightarrow>
-       combine_abs (env c) (env ex) \<le> env ret"
+       \<langle>env c|env ex\<rangle> \<le> env ret"
   assumes entry_le: "s0 \<le> env (cfg_entry g)"
-  shows "cfg_collect g S v0 \<le> gamma_state (env v0)"
+  shows "cfg_collect g S v0 \<le> \<lbrakk>env v0\<rbrakk>"
 proof -
   have paths: "cfg_collect g S v0 \<subseteq> cfg_collect_paths g S v0"
     by (rule cfg_collect_le_paths)
@@ -258,7 +260,7 @@ proof -
     assume "t \<in> cfg_collect g S v0"
     with paths have wit: "cfg_witness g S v0 t"
       unfolding cfg_collect_paths_def by auto
-    show "t \<in> gamma_state (env v0)"
+    show "t \<in> \<lbrakk>env v0\<rbrakk>"
       using S_sound combine_le entry_le fin finC cfg_witness_gamma step_le wit by blast
   qed
 qed
@@ -267,28 +269,28 @@ theorem post_fixpoint_sound:
   assumes fin: "finite (edges g)"
   assumes finC: "finite (combines g)"
   assumes post_fp: "is_post_fixpoint g tf (\<squnion>) bot s0 env"
-  assumes S_sound: "S \<le> gamma_state s0"
-  shows "\<forall>v. cfg_collect g S v \<le> gamma_state (env v)"
+  assumes S_sound: "S \<le> \<lbrakk>s0\<rbrakk>"
+  shows "\<forall>v. cfg_collect g S v \<le> \<lbrakk>env v\<rbrakk>"
 proof -
-  have coll_le: "\<And>v. collect_pp g (\<lambda>v. gamma_state (env v)) v \<le> gamma_state (env v)"
+  have coll_le: "\<And>v. collect_pp g (\<lambda>v. \<lbrakk>env v\<rbrakk>) v \<le> \<lbrakk>env v\<rbrakk>"
     by (rule collect_pp_abstract_sound[OF fin finC post_fp])
-  have comb_le: "\<And>v. collect_combine_pp g (\<lambda>v. gamma_state (env v)) v
-                  \<le> gamma_state (env v)"
+  have comb_le: "\<And>v. collect_combine_pp g (\<lambda>v. \<lbrakk>env v\<rbrakk>) v
+                  \<le> \<lbrakk>env v\<rbrakk>"
     by (rule collect_combine_pp_abstract_sound[OF fin finC post_fp])
   have s0_le_env: "s0 \<le> env (cfg_entry g)"
     using s0_le_rhs_entry[OF fin finC]
           post_fp[unfolded is_post_fixpoint_def, rule_format, of "cfg_entry g"]
     by (rule order_trans)
-  have S_le_env: "S \<le> gamma_state (env (cfg_entry g))"
+  have S_le_env: "S \<le> \<lbrakk>env (cfg_entry g)\<rbrakk>"
     using S_sound gamma_state_mono[OF s0_le_env] by blast
-  have key: "cfg_collect_F g S (\<lambda>v. gamma_state (env v)) \<le> (\<lambda>v. gamma_state (env v))"
+  have key: "cfg_collect_F g S (\<lambda>v. \<lbrakk>env v\<rbrakk>) \<le> (\<lambda>v. \<lbrakk>env v\<rbrakk>)"
   proof (rule le_funI)
     fix v
-    show "cfg_collect_F g S (\<lambda>v. gamma_state (env v)) v \<le> gamma_state (env v)"
+    show "cfg_collect_F g S (\<lambda>v. \<lbrakk>env v\<rbrakk>) v \<le> \<lbrakk>env v\<rbrakk>"
       unfolding cfg_collect_F_def
       using coll_le comb_le S_le_env by auto
   qed
-  have "cfg_collect g S \<le> (\<lambda>v. gamma_state (env v))"
+  have "cfg_collect g S \<le> (\<lambda>v. \<lbrakk>env v\<rbrakk>)"
     unfolding cfg_collect_def
     by (simp add: key lfp_lowerbound)
   then show ?thesis by (auto simp: le_fun_def)
@@ -297,3 +299,4 @@ qed
 end
 
 end
+
